Semantic/Consume/TypeSystem/BasicProps.lean
@@ -48,22 +48,24 @@ theorem Ctx.lookup_tvar_det {Γ : Ctx s} {X : BVar s .tvar} {T1 T2 : PureTy s} :
       exact ih h2'
 
 theorem Ctx.lookup_cvar_det {Γ : Ctx s} {c : BVar s .cvar} {m1 m2 : UseMode}
-    {cb1 cb2 : CaptureBound s} :
-    Γ.LookupCVar c m1 cb1 -> Γ.LookupCVar c m2 cb2 -> m1 = m2 ∧ cb1 = cb2 := by
+    {cb1 cb2 : CaptureBound s} {locked1 locked2 : Bool} :
+    Γ.LookupCVar c m1 cb1 locked1 -> Γ.LookupCVar c m2 cb2 locked2 ->
+    m1 = m2 ∧ cb1 = cb2 ∧ locked1 = locked2 := by
   intro h1 h2
-  induction h1
+  induction h1 generalizing m2 locked2
   case here =>
     cases h2
-    case here => exact ⟨rfl, rfl⟩
+    case here => exact ⟨rfl, rfl, rfl⟩
   case there ih =>
     cases h2
     case there h2' =>
-      obtain ⟨hm, hcb⟩ := ih h2'
-      exact ⟨hm, by rw [hcb]⟩
+      obtain ⟨hm, hcb, hlk⟩ := ih h2'
+      exact ⟨hm, by rw [hcb], hlk⟩
   case lock ih =>
     cases h2
     case lock h2' =>
-      exact ih h2'
+      obtain ⟨hm, hcb, _⟩ := ih h2'
+      exact ⟨hm, hcb, rfl⟩
 
 -- Subsumption reflexivity
 
